WIP `getOType` and `getWType` instructions: mainly needs to fix iInstr

theories/rules/rules_Get.v
@@ -11,6 +11,7 @@ Section cap_lang_rules.
   Implicit Types σ : ExecConf.
   Implicit Types c : cap_lang.expr.
   Implicit Types a b : Addr.
+  Implicit Types o : OType.
   Implicit Types r : RegName.
   Implicit Types v : cap_lang.val.
   Implicit Types w : Word.
@@ -21,22 +22,38 @@ Section cap_lang_rules.
   Definition denote (i: instr) (w : Word): option Z :=
     match w with
     | WCap p b e a =>
-      match i with
-      | GetP _ _ => Some (encodePerm p)
-      | GetB _ _ => Some (b:Z)
-      | GetE _ _ => Some (e:Z)
-      | GetA _ _ => Some (a:Z)
-      | _ => None
-      end
+        match i with
+        | GetP _ _ => Some (encodePerm p)
+        | GetB _ _ => Some (b:Z)
+        | GetE _ _ => Some (e:Z)
+        | GetA _ _ => Some (a:Z)
+        | GetOType _ _ => Some (-1)%Z
+        | GetWType _ _ => Some (encodeWordType w)
+        | _ => None
+        end
     | WSealRange p b e a =>
-      match i with
-      | GetP _ _ => Some (encodeSealPerms p)
-      | GetB _ _ => Some (b:Z)
-      | GetE _ _ => Some (e:Z)
-      | GetA _ _ => Some (a:Z)
-      | _ => None
-      end
-    | _ => None end.
+        match i with
+        | GetP _ _ => Some (encodeSealPerms p)
+        | GetB _ _ => Some (b:Z)
+        | GetE _ _ => Some (e:Z)
+        | GetA _ _ => Some (a:Z)
+        | GetOType _ _ => Some (-1)%Z
+        | GetWType _ _ => Some (encodeWordType w)
+        | _ => None
+        end
+    | WSealed o _ =>
+        match i with
+        | GetOType _ _ => Some (o:Z)
+        | GetWType _ _ => Some (encodeWordType w)
+        | _ => None
+        end
+    | WInt _ =>
+        match i with
+        | GetOType _ _ => Some (-1)%Z
+        | GetWType _ _ => Some (encodeWordType w)
+        | _ => None
+        end
+    end.
 
   Global Arguments denote : simpl nomatch.
 
@@ -44,7 +61,10 @@ Section cap_lang_rules.
     i = GetP dst src ∨
     i = GetB dst src ∨
     i = GetE dst src ∨
-    i = GetA dst src.
+    i = GetA dst src \/
+    i = GetOType dst src \/
+    i = GetWType dst src
+  .
 
   Lemma regs_of_is_Get i dst src :
     is_Get i dst src →
@@ -60,10 +80,12 @@ Section cap_lang_rules.
       | GetB _ _ => b
       | GetE _ _ => e
       | GetA _ _ => a
+      | GetOType _ _ => (-1)%Z
+      | GetWType _ _ => (encodeWordType (WCap p b e a))
       | _ => 0%Z
       end.
   Lemma denote_cap_denote i p b e a z src dst: is_Get i src dst → denote_cap i p b e a = z → denote i (WCap p b e a) = Some z.
-  Proof. unfold denote_cap, denote, is_Get. intros [-> | [-> | [-> | ->]]] ->; done. Qed.
+  Proof. unfold denote_cap, denote, is_Get. intros [-> | [-> | [-> | [-> | [-> | ->]]]]] ->; done. Qed.
 
   Definition denote_seal (i: instr) (p : SealPerms) (b e a : OType): Z :=
       match i with
@@ -71,10 +93,33 @@ Section cap_lang_rules.
       | GetB _ _ => b
       | GetE _ _ => e
       | GetA _ _ => a
+      | GetOType _ _ => (-1)%Z
+      | GetWType _ _ => (encodeWordType (WSealRange p b e a))
       | _ => 0%Z
       end.
   Lemma denote_seal_denote i (p : SealPerms) (b e a : OType) z src dst: is_Get i src dst → denote_seal i p b e a = z → denote i (WSealRange p b e a) = Some z.
-  Proof. unfold denote_seal, denote, is_Get. intros [-> | [-> | [-> | ->]]] ->; done. Qed.
+  Proof. unfold denote_seal, denote, is_Get. intros [-> | [-> | [-> | [-> | [-> | ->]]]]] ->; done. Qed.
+
+  Lemma denote_wtype w dst src : denote (GetWType dst src) w
+                                 = Some (encodeWordType w).
+  Proof.
+    unfold denote ; destruct w ; cycle 1 ; [destruct sb|..]; auto.
+  Qed.
+  (* Definition denote_sealed (i: instr) (o : OType) (s : Sealable) : Z := *)
+  (*     match i with *)
+  (*     | GetOType _ _ => o *)
+  (*     | GetWType _ _ => (encodeWordType (WSealed o s)) *)
+  (*     | _ => 0%Z *)
+  (*     end. *)
+  (* Lemma denote_sealed_denote i (o : OType) (s : Sealable) z src dst : is_Get i src dst → denote_sealed i o s = z → denote i (WSealed o s) = Some z. *)
+  (* Proof. unfold denote_sealed, denote, is_Get. *)
+  (*        intros. *)
+  (*        destruct H2 as [-> |]. *)
+  (*        intros [-> | [-> | [-> | [-> | [-> | ->]]]]]. ->; done. Qed. *)
+  (* Proof. unfold denote_sealed, denote, is_Get. *)
+  (*        intros [ -> | -> ]. *)
+  (*        intros *)
+  (*          [-> | [-> | [-> | [-> | [-> | ->]]]]] ->; done. Qed. *)
 
   Inductive Get_failure (i: instr) (regs: Reg) (dst src: RegName) :=
     | Get_fail_src_denote w:
@@ -176,7 +221,7 @@ Section cap_lang_rules.
     isCorrectPC (WCap pc_p pc_b pc_e pc_a) →
     (pc_a + 1)%a = Some pc_a' ->
     denote get_i (WCap pc_p pc_b pc_e pc_a) = Some z →
-    
+
     {{{ ▷ PC ↦ᵣ WCap pc_p pc_b pc_e pc_a
         ∗ ▷ pc_a ↦ₐ w
         ∗ ▷ dst ↦ᵣ wdst }}}
@@ -278,7 +323,13 @@ Proof. intros; unfold is_Get; eauto. Qed.
 Lemma is_Get_GetA dst src : is_Get (GetA dst src) dst src.
 Proof. intros; unfold is_Get; eauto. Qed.
 
+Lemma is_Get_GetOType dst src : is_Get (GetOType dst src) dst src.
+Proof. intros; unfold is_Get; eauto; firstorder. Qed.
+Lemma is_Get_GetWType dst src : is_Get (GetWType dst src) dst src.
+Proof. intros; unfold is_Get; eauto; firstorder. Qed.
 Global Hint Resolve is_Get_GetP : core.
 Global Hint Resolve is_Get_GetB : core.
 Global Hint Resolve is_Get_GetE : core.
 Global Hint Resolve is_Get_GetA : core.
+Global Hint Resolve is_Get_GetOType : core.
+Global Hint Resolve is_Get_GetWType : core.
