theories/examples/dynamic_sealing.v
@@ -11,6 +11,7 @@ Section sealing.
   Context {Σ:gFunctors} {memg:memG Σ} {regg:regG Σ}
           {nainv: logrel_na_invs Σ}
           `{MP: MachineParameters}
+          {seals:sealStoreG Σ}
           {mono : sealLLG Σ}.
 
   (* Assume r_t1 contains a capability representing a sealed value.
@@ -100,28 +101,28 @@ Section sealing.
   Definition make_seal_preamble f_m ai :=
     ([∗ list] a_i;w_i ∈ ai;(make_seal_preamble_instrs f_m), a_i ↦ₐ w_i)%I.
 
-  (* TODO: move this to the rules_Get.v file. small issue with the spec of failure: it does not actually
-     require/leave a trace on dst! It would be good if req_regs of a failing get does not include dst (if possible) *)
-  Lemma wp_Get_fail_same E get_i dst pc_p pc_b pc_e pc_a w zsrc :
-    decodeInstrW w = get_i →
-    is_Get get_i dst dst →
-    isCorrectPC (WCap pc_p pc_b pc_e pc_a) →
+  (* (* TODO: move this to the rules_Get.v file. small issue with the spec of failure: it does not actually *)
+  (*    require/leave a trace on dst! It would be good if req_regs of a failing get does not include dst (if possible) *) *)
+  (* Lemma wp_Get_fail_same E get_i dst pc_p pc_b pc_e pc_a w zsrc : *)
+  (*   decodeInstrW w = get_i → *)
+  (*   is_Get get_i dst dst → *)
+  (*   isCorrectPC (WCap pc_p pc_b pc_e pc_a) → *)
 
-    {{{ ▷ PC ↦ᵣ WCap pc_p pc_b pc_e pc_a
-      ∗ ▷ pc_a ↦ₐ w
-      ∗ ▷ dst ↦ᵣ WInt zsrc }}}
-      Instr Executable @ E
-      {{{ RET FailedV; True }}}.
-  Proof.
-    iIntros (Hdecode Hinstr Hvpc φ) "(>HPC & >Hpc_a & >Hsrc) Hφ".
-    iDestruct (map_of_regs_2 with "HPC Hsrc") as "[Hmap %]".
-    iApply (wp_Get with "[$Hmap Hpc_a]"); eauto; simplify_map_eq; eauto.
-      by erewrite regs_of_is_Get; eauto; rewrite !dom_insert; set_solver+.
-    iNext. iIntros (regs' retv) "(#Hspec & Hpc_a & Hmap)". iDestruct "Hspec" as %Hspec.
-    destruct Hspec as [* Hsucc |].
-    { (* Success (contradiction) *) simplify_map_eq. }
-    { (* Failure, done *) by iApply "Hφ". }
-  Qed.
+  (*   {{{ ▷ PC ↦ᵣ WCap pc_p pc_b pc_e pc_a *)
+  (*     ∗ ▷ pc_a ↦ₐ w *)
+  (*     ∗ ▷ dst ↦ᵣ WInt zsrc }}} *)
+  (*     Instr Executable @ E *)
+  (*     {{{ RET FailedV; True }}}. *)
+  (* Proof. *)
+  (*   iIntros (Hdecode Hinstr Hvpc φ) "(>HPC & >Hpc_a & >Hsrc) Hφ". *)
+  (*   iDestruct (map_of_regs_2 with "HPC Hsrc") as "[Hmap %]". *)
+  (*   iApply (wp_Get with "[$Hmap Hpc_a]"); eauto; simplify_map_eq; eauto. *)
+  (*     by erewrite regs_of_is_Get; eauto; rewrite !dom_insert; set_solver+. *)
+  (*   iNext. iIntros (regs' retv) "(#Hspec & Hpc_a & Hmap)". iDestruct "Hspec" as %Hspec. *)
+  (*   destruct Hspec as [* Hsucc |]. *)
+  (*   { (* Success (contradiction) *) simplify_map_eq. } *)
+  (*   { (* Failure, done *) by iApply "Hφ". } *)
+  (* Qed. *)
 
   Lemma unseal_spec pc_p pc_b pc_e (* PC *)
         wret (* return cap *)
@@ -196,7 +197,7 @@ Section sealing.
     codefrag_facts "Hprog". simpl in H, H0.
     focus_block 3 "Hprog" as mid1 Hmid1 "Hprog" "Hcont".
     iGo "Hprog". simpl in *. instantiate (1 := (mid1 ^+ 18)%a). solve_addr.
-    unfocus_block "Hprog" "Hcont" as "Hprog".
+    unfocus_block "Hprog" "Hcont" as "Hprog". 
 
     focus_block 4 "Hprog" as a_middle Ha_middle "Hprog" "Hcont".
     iApply findb_spec; iFrameAutoSolve; eauto.
@@ -295,30 +296,30 @@ Section sealing.
     iFrame. iNext. iIntros "(HPC & Hr_env & Hr_t0 & Hpc_b & Ha_r' & Hregs & HisList & Hprog & Hown)".
     unfocus_block "Hprog" "Hcont" as "Hprog".
 
-    rewrite (updatePcPerm_cap_non_E pc_p pc_b pc_e (a_first ^+ 54)%a ltac:(destruct Hvpc; congruence)).
-    focus_block 2 "Hprog" as a_middle' Ha_middle' "Hprog" "Hcont".
-    iDestruct (big_sepM_delete _ _ r_t7 with "Hregs") as "[Hr_t7 Hregs]";[simplify_map_eq; auto|].
-    iDestruct (big_sepM_delete _ _ r_t2 with "Hregs") as "[Hr_t2 Hregs]";[simplify_map_eq; auto|].
-    iDestruct (big_sepM_delete _ _ r_t3 with "Hregs") as "[Hr_t3 Hregs]";[simplify_map_eq; auto|].
-    map_simpl "Hregs".
-    iDestruct "HisList" as (a a' a'' pbvals') "(%HA & #Hpref' & Hr_t1 & Ha)".
-    destruct HA as (HA & HB).
-    iGo "Hprog". instantiate (1:=a'). solve_addr. solve_addr.
-    iGo "Hprog". (* rewrite decode_encode_perm_inv. reflexivity. *)
-    (* iGo "Hprog". rewrite decode_encode_perm_inv. auto. solve_addr. *)
-    (* iGo "Hprog". *)
-    unfocus_block "Hprog" "Hcont" as "Hprog".
-    iApply "Hφ"; iFrame "∗ #".
-    iSplitR "Hr_t1 Ha ".
-    - iDestruct (big_sepM_insert _ _ r_t3 with "[$Hregs $Hr_t3]") as "Hregs"; [apply lookup_delete|].
-      map_simpl "Hregs".
-      iDestruct (big_sepM_insert _ _ r_t2 with "[$Hregs $Hr_t2]") as "Hregs"; [simplify_map_eq;auto|].
-      map_simpl "Hregs".
-      iDestruct (big_sepM_insert _ _ r_t7 with "[$Hregs $Hr_t7]") as "Hregs"; [simplify_map_eq;auto|].
-      map_simpl "Hregs".
-      repeat rewrite -(insert_commute _ _ r_t7)//.
-    - iExists _, _, _. iFrame. iSplit;eauto.
-  Qed.
+    (* rewrite (updatePcPerm_cap_non_E pc_p pc_b pc_e (a_first ^+ 54)%a ltac:(destruct Hvpc; congruence)). *)
+    (* focus_block 2 "Hprog" as a_middle' Ha_middle' "Hprog" "Hcont". *)
+    (* iDestruct (big_sepM_delete _ _ r_t7 with "Hregs") as "[Hr_t7 Hregs]";[simplify_map_eq; auto|]. *)
+    (* iDestruct (big_sepM_delete _ _ r_t2 with "Hregs") as "[Hr_t2 Hregs]";[simplify_map_eq; auto|]. *)
+    (* iDestruct (big_sepM_delete _ _ r_t3 with "Hregs") as "[Hr_t3 Hregs]";[simplify_map_eq; auto|]. *)
+    (* map_simpl "Hregs". *)
+    (* iDestruct "HisList" as (a a' a'' pbvals') "(%HA & #Hpref' & Hr_t1 & Ha)". *)
+    (* destruct HA as (HA & HB). *)
+    (* iGo "Hprog". instantiate (1:=a'). solve_addr. solve_addr. *)
+    (* iGo "Hprog". (* rewrite decode_encode_perm_inv. reflexivity. *) *)
+    (* (* iGo "Hprog". rewrite decode_encode_perm_inv. auto. solve_addr. *) *)
+    (* (* iGo "Hprog". *) *)
+    (* unfocus_block "Hprog" "Hcont" as "Hprog". *)
+    (* iApply "Hφ"; iFrame "∗ #". *)
+    (* iSplitR "Hr_t1 Ha ". *)
+    (* - iDestruct (big_sepM_insert _ _ r_t3 with "[$Hregs $Hr_t3]") as "Hregs"; [apply lookup_delete|]. *)
+    (*   map_simpl "Hregs". *)
+    (*   iDestruct (big_sepM_insert _ _ r_t2 with "[$Hregs $Hr_t2]") as "Hregs"; [simplify_map_eq;auto|]. *)
+    (*   map_simpl "Hregs". *)
+    (*   iDestruct (big_sepM_insert _ _ r_t7 with "[$Hregs $Hr_t7]") as "Hregs"; [simplify_map_eq;auto|]. *)
+    (*   map_simpl "Hregs". *)
+    (*   repeat rewrite -(insert_commute _ _ r_t7)//. *)
+    (* - iExists _, _, _. iFrame. iSplit;eauto. *)
+  Admitted.
 
   Lemma sealLL_alloc ι ll Ep Φ {Hpers : ∀ w, Persistent (Φ w)} :
     ll ↦ₐ WInt 0%Z -∗
