theories/fundamental_binary.v
@@ -1,7 +1,7 @@
 From iris.proofmode Require Import proofmode.
 From iris.program_logic Require Import weakestpre adequacy lifting.
 From stdpp Require Import base.
-From cap_machine.ftlr_binary Require Export Mov_binary Load_binary AddSubLt_binary Get_binary GetTag_binary GetSealed_binary IsCap_binary GetTag_binary Jmp_binary Jnz_binary Lea_binary Subseg_binary Restrict_binary Store_binary Seal_binary UnSeal_binary.
+From cap_machine.ftlr_binary Require Export Mov_binary Load_binary AddSubLt_binary Get_binary Jmp_binary Jnz_binary Lea_binary Subseg_binary Restrict_binary Store_binary Seal_binary UnSeal_binary.
 From cap_machine Require Export logrel_binary.
 
 Section bin_log_def.
@@ -96,9 +96,8 @@ Section fundamental.
       + (* GetE *) iApply (get_case with "[] [] [] [] [] [] [Hsreg] [Hown] [Hs] [Ha] [Ha'] [HP] [Hcls] [HPC] [Hmap]"); try (eapply Hi); try iAssumption; eauto.
       + (* GetA *) iApply (get_case with "[] [] [] [] [] [] [Hsreg] [Hown] [Hs] [Ha] [Ha'] [HP] [Hcls] [HPC] [Hmap]"); try (eapply Hi); try iAssumption; eauto.
       + (* GetP *) iApply (get_case with "[] [] [] [] [] [] [Hsreg] [Hown] [Hs] [Ha] [Ha'] [HP] [Hcls] [HPC] [Hmap]"); try (eapply Hi); try iAssumption; eauto.
-      + (* IsCap *) iApply (iscap_case with "[] [] [] [] [] [] [Hsreg] [Hown] [Hs] [Ha] [Ha'] [HP] [Hcls] [HPC] [Hmap]"); try iAssumption; eauto.
-      + (* GetTag *) iApply (get_tag_case with "[] [] [] [] [] [] [Hsreg] [Hown] [Hs] [Ha] [Ha'] [HP] [Hcls] [HPC] [Hmap]"); try iAssumption; eauto.
-      + (* GetSealed *) iApply (get_sealed_case with "[] [] [] [] [] [] [Hsreg] [Hown] [Hs] [Ha] [Ha'] [HP] [Hcls] [HPC] [Hmap]"); try iAssumption; eauto.
+      + (* GetWType *) iApply (get_case with "[] [] [] [] [] [] [Hsreg] [Hown] [Hs] [Ha] [Ha'] [HP] [Hcls] [HPC] [Hmap]"); try (eapply Hi); try iAssumption; eauto.
+      + (* GetOType *) iApply (get_case with "[] [] [] [] [] [] [Hsreg] [Hown] [Hs] [Ha] [Ha'] [HP] [Hcls] [HPC] [Hmap]"); try (eapply Hi); try iAssumption; eauto.
       + (* Seal *) iApply (seal_case with "[] [] [] [] [] [] [Hsreg] [Hown] [Hs] [Ha] [Ha'] [HP] [Hcls] [HPC] [Hmap]"); try (eapply Hi); try iAssumption; eauto.
       + (* UnSeal *) iApply (unseal_case with "[] [] [] [] [] [] [Hsreg] [Hown] [Hs] [Ha] [Ha'] [HP] [Hcls] [HPC] [Hmap]"); try (eapply Hi); try iAssumption; eauto.
       + (* Fail *)
