theories/machine_base.v
@@ -52,12 +52,9 @@ Inductive instr: Type :=
 | GetB (dst r: RegName)
 | GetE (dst r: RegName)
 | GetA (dst r: RegName)
-| GetP (dst r: RegName) (* corresponds to CGetPerm in CHERI MIPS *)
-| IsCap (dst r: RegName) (* previously IsPtr *)
-| GetTag (dst r: RegName) (* corresponds to CGetTag in CHERI MIPS *)
-| GetSealed (dst r: RegName) (* corresponds to CGetSealed in CHERI MIPS *)
-(* GetType could replace GetSealed, but we need a way to convert otype -> Z *)
-(* | GetType (dst r: RegName) *)
+| GetP (dst r: RegName)
+| GetWType (dst r : RegName) (* combine IsCap, GetTage and GetSealed all together into a unique encoding *)
+| GetOType (dst r: RegName)
 | Seal (dst : RegName) (r1 r2: RegName)
 | UnSeal (dst : RegName) (r1 r2: RegName)
 | Fail
@@ -728,15 +725,13 @@ Proof.
       | GetA dst r => GenNode 13 [GenLeaf (inl dst); GenLeaf (inl r)]
       | GetP dst r => GenNode 14 [GenLeaf (inl dst); GenLeaf (inl r)]
 
-      | GetTag dst r => GenNode 15 [GenLeaf (inl dst); GenLeaf (inl r)]
-      | GetSealed dst r => GenNode 16 [GenLeaf (inl dst); GenLeaf (inl r)]
-      (* | GetType dst r => GenNode 16 [GenLeaf (inl dst); GenLeaf (inl r)] *)
-      | IsCap dst r => GenNode 17 [GenLeaf (inl dst); GenLeaf (inl r)]
+      | GetOType dst r => GenNode 15 [GenLeaf (inl dst); GenLeaf (inl r)]
+      | GetWType dst r => GenNode 16 [GenLeaf (inl dst); GenLeaf (inl r)]
 
-      | Seal dst r1 r2 => GenNode 18 [GenLeaf (inl dst); GenLeaf (inl r1); GenLeaf (inl r2)]
-      | UnSeal dst r1 r2 => GenNode 19 [GenLeaf (inl dst); GenLeaf (inl r1); GenLeaf (inl r2)]
-      | Fail => GenNode 20 []
-      | Halt => GenNode 21 []
+      | Seal dst r1 r2 => GenNode 17 [GenLeaf (inl dst); GenLeaf (inl r1); GenLeaf (inl r2)]
+      | UnSeal dst r1 r2 => GenNode 18 [GenLeaf (inl dst); GenLeaf (inl r1); GenLeaf (inl r2)]
+      | Fail => GenNode 19 []
+      | Halt => GenNode 20 []
       end).
   set (dec := fun e =>
       match e with
@@ -756,15 +751,13 @@ Proof.
       | GenNode 13 [GenLeaf (inl dst); GenLeaf (inl r)] => GetA dst r
       | GenNode 14 [GenLeaf (inl dst); GenLeaf (inl r)] => GetP dst r
 
-      | GenNode 15 [GenLeaf (inl dst); GenLeaf (inl r)] => GetTag dst r
-      | GenNode 16 [GenLeaf (inl dst); GenLeaf (inl r)] => GetSealed dst r
-      | GenNode 17 [GenLeaf (inl dst); GenLeaf (inl r)] => IsCap dst r
-      (* | GenNode 16 [GenLeaf (inl dst); GenLeaf (inl r)] => GetType dst r *)
+      | GenNode 15 [GenLeaf (inl dst); GenLeaf (inl r)] => GetOType dst r
+      | GenNode 16 [GenLeaf (inl dst); GenLeaf (inl r)] => GetWType dst r
 
-      | GenNode 18 [GenLeaf (inl dst); GenLeaf (inl r1); GenLeaf (inl r2)] => Seal dst r1 r2
-      | GenNode 19 [GenLeaf (inl dst); GenLeaf (inl r1); GenLeaf (inl r2)] => UnSeal dst r1 r2
-      | GenNode 20 [] => Fail
-      |  GenNode 21 [] => Halt
+      | GenNode 17 [GenLeaf (inl dst); GenLeaf (inl r1); GenLeaf (inl r2)] => Seal dst r1 r2
+      | GenNode 18 [GenLeaf (inl dst); GenLeaf (inl r1); GenLeaf (inl r2)] => UnSeal dst r1 r2
+      | GenNode 19 [] => Fail
+      |  GenNode 20 [] => Halt
       | _ => Fail (* dummy *)
       end).
   refine (inj_countable' enc dec _).
