theories/machine_parameters.v
@@ -3,26 +3,41 @@ From stdpp Require Import base.
 From cap_machine Require Export machine_base.
 
 Class MachineParameters := {
-  decodeInstr : Z → instr;
-  encodeInstr : instr → Z;
+    decodeInstr : Z → instr;
+    encodeInstr : instr → Z;
 
-  decode_encode_instr_inv :
+    decode_encode_instr_inv :
     forall (i: instr), decodeInstr (encodeInstr i) = i;
 
-  encodePerm : Perm → Z;
-  encodePerm_inj : Inj eq eq encodePerm;
-  decodePerm : Z → Perm;
+    encodePerm : Perm → Z;
+    encodePerm_inj : Inj eq eq encodePerm;
+    decodePerm : Z → Perm;
 
-  decode_encode_perm_inv :
+    decode_encode_perm_inv :
     forall pl, decodePerm (encodePerm pl) = pl;
 
-  encodeSealPerms : SealPerms → Z;
-  encodeSealPerms_inj : Inj eq eq encodeSealPerms;
-  decodeSealPerms : Z → SealPerms;
+    encodeSealPerms : SealPerms → Z;
+    encodeSealPerms_inj : Inj eq eq encodeSealPerms;
+    decodeSealPerms : Z → SealPerms;
 
-  decode_encode_seal_perms_inv :
+    decode_encode_seal_perms_inv :
     forall pl, decodeSealPerms (encodeSealPerms pl) = pl;
-}.
+
+    encodeWordType : Word -> Z;
+    decodeWordType : Z -> Word;
+    encodeWordType_correct :
+    forall w w', match w,w' with
+            | WCap _ _ _ _, WCap _ _ _ _ => encodeWordType w = encodeWordType w'
+            | WSealRange _ _ _ _, WSealRange _ _ _ _ => encodeWordType w = encodeWordType w'
+            | WSealed _ _, WSealed _ _ => encodeWordType w = encodeWordType w'
+            | WInt _, WInt _ => encodeWordType w = encodeWordType w'
+            | _, _ =>encodeWordType w <> encodeWordType w'
+            end;
+    decode_encode_word_type_inv :
+    forall w, decodeWordType (encodeWordType w) = w;
+    (* TODO I think that we need more hypetheses about the encoding/decoding of
+     word type: we do need some sort injectivity, modulo word type *)
+  }.
 
 (* Lift the encoding / decoding between Z and instructions on Words: simplify
    fail on capabilities. *)
@@ -43,3 +58,41 @@ Proof. apply decode_encode_instr_inv. Qed.
 
 Definition encodeInstrsW `{MachineParameters} : list instr → list Word :=
   map encodeInstrW.
+
+(* TODO solve_encodeWordType tactic ?*)
+Lemma encodeWordType_correct_cap `{MachineParameters} : forall p b e a p' b' e' a',
+  encodeWordType (WCap p b e a) = encodeWordType (WCap p' b' e' a').
+  intros
+  ; match goal with
+    | H: _ |- encodeWordType ?x = encodeWordType ?y =>
+        pose proof (encodeWordType_correct x y) as Heq ; simpl in Heq ; auto
+    end.
+Qed.
+
+Lemma encodeWordType_correct_int `{MachineParameters} : forall z z',
+  encodeWordType (WInt z) = encodeWordType (WInt z').
+  intros
+  ; match goal with
+    | H: _ |- encodeWordType ?x = encodeWordType ?y =>
+        pose proof (encodeWordType_correct x y) as Heq ; simpl in Heq ; auto
+    end.
+Qed.
+
+Lemma encodeWordType_correct_sealrange `{MachineParameters} : forall p b e a p' b' e' a',
+  encodeWordType (WSealRange p b e a) = encodeWordType (WSealRange p' b' e' a').
+Proof.
+  intros
+  ; match goal with
+    | H: _ |- encodeWordType ?x = encodeWordType ?y =>
+        pose proof (encodeWordType_correct x y) as Heq ; simpl in Heq ; auto
+    end.
+Qed.
+
+Lemma encodeWordType_correct_sealed `{MachineParameters} : forall o s o' s',
+  encodeWordType (WSealed o s) = encodeWordType (WSealed o' s').
+  intros
+  ; match goal with
+    | H: _ |- encodeWordType ?x = encodeWordType ?y =>
+        pose proof (encodeWordType_correct x y) as Heq ; simpl in Heq ; auto
+    end.
+Qed.
