theories/rules.v
@@ -1,7 +1,7 @@
 From cap_machine.rules Require Export
      rules_Get rules_Load rules_Store rules_AddSubLt
-     rules_Lea rules_Mov rules_Restrict rules_GetTag rules_GetSealed rules_IsCap
-     rules_Jmp rules_Jnz rules_Subseg rules_Seal rules_UnSeal.
+     rules_Lea rules_Mov rules_Restrict rules_Jmp rules_Jnz rules_Subseg
+     rules_Seal rules_UnSeal.
 From iris.base_logic Require Export invariants gen_heap.
 From iris.program_logic Require Export weakestpre ectx_lifting.
 From cap_machine.rules Require Export rules_base.
